## Анализ миноров

$$
\det S = \begin{vmatrix}
A_1 & A_2 & A_3 & A_0 & 0 & 0\\
0 & A_1 & A_2 & A_3 & A_0 & 0\\ 
0 & 0 & A_1 & A_2 & A_3 & A_0\\
B_1 & B_2 & B_3 & B_0 & 0 & 0\\
0 & B_1 & B_2 & B_3 & B_0 & 0\\ 
0 & 0 & B_1 & B_2 & B_3 & B_0
\end{vmatrix}$$

$$
\begin{gathered}

\bar{M}_{1,2,3} = M_{4,5,6}
= \begin{vmatrix}
B_1 & B_2 & B_3\\
0   & B_1 & B_2\\ 
0   & 0   & B_1
\end{vmatrix}
= B_1^3
;\\
\bar{M}_{1,2,6} = M_{3,4,5} 
= \begin{vmatrix}
0   & 0   & A_1\\
B_1 & B_2 & B_3\\
0   & B_1 & B_2 
\end{vmatrix}
= A_1 B_1^2
;\\
\bar{M}_{1,3,5} = M_{2,4,6}
= \begin{vmatrix}
0   & A_1 & A_2\\ 
B_1 & B_2 & B_3\\
0   & 0   & B_1
\end{vmatrix}
= - A_1 B_1^2
; \\

\bar{M}_{1,3,6} = M_{2,4,5}
= \begin{vmatrix}
0   & A_1 & A_2\\ 
B_1 & B_2 & B_3\\
0   & B_1 & B_2 
\end{vmatrix}
= -B_1 (A_1B_2 - A_2B_1)
;\\
\bar{M}_{1,5,6} = M_{2,3,4}
= \begin{vmatrix}
0   & A_1 & A_2\\ 
0   & 0   & A_1\\
B_1 & B_2 & B_3
\end{vmatrix}
= B_1 A_1^2
;\\
\bar{M}_{2,3,4} = M_{1,5,6}
=\begin{vmatrix}
A_1 & A_2 & A_3\\
0   & B_1 & B_2\\ 
0   & 0   & B_1
\end{vmatrix}
=A_1 B_1^2
;\\
\bar{M}_{2,3,5} = M_{1,4,6}
= \begin{vmatrix}
A_1 & A_2 & A_3\\
B_1 & B_2 & B_3\\
0   & 0   & B_1
\end{vmatrix}
= B_1(A_1B_2 - A_2B_1)
;\\
\bar{M}_{2,3,6} = M_{1,4,5}
= \begin{vmatrix}
A_1 & A_2 & A_3\\
B_1 & B_2 & B_3\\
0   & B_1 & B_2 
\end{vmatrix}
= A_1(B_2^2-B_1B_3) - B_1(A_2B_2-A_3B_1)
;\\
\bar{M}_{2,4,6} = M_{1,3,5}
=\begin{vmatrix}
A_1 & A_2 & A_3\\
0   & 0   & A_1\\
0   & B_1 & B_2 
\end{vmatrix}
=-A_1^2 B_1
;\\
\bar{M}_{2,5,6} = M_{1,3,4}
=\begin{vmatrix}
A_1 & A_2 & A_3\\
0   & 0   & A_1\\
B_1 & B_2 & B_3
\end{vmatrix}
=-A_1(A_1 B_2 - A_2 B_1)
;\\
\bar{M}_{3,4,5} = M_{1,2,6}
=\begin{vmatrix}
A_1 & A_2 & A_3\\
0   & A_1 & A_2\\ 
0   & 0   & B_1
\end{vmatrix}
= A_1^2 B^1
;\\
\bar{M}_{3,4,6} = M_{1,2,5}
=\begin{vmatrix}
A_1 & A_2 & A_3\\
0   & A_1 & A_2\\ 
0   & B_1 & B_2
\end{vmatrix}
=A_1 (A_1 B_2 - A_2 B_1)
;\\
\bar{M}_{3,5,6} = M_{1,2,4}
=\begin{vmatrix}
A_1 & A_2 & A_3\\
0   & A_1 & A_2\\ 
B_1 & B_2 & B_3
\end{vmatrix}
= A_1 (A_1B_3 - A_2 B_2) + B_1(A_2^2 - A_1 A_3)
;\\
\bar{M}_{4,5,6} = M_{1,2,3}
=\begin{vmatrix}
A_1 & A_2 & A_3\\
0   & A_1 & A_2\\ 
0   & 0   & A_1
\end{vmatrix}
= A_1 ^3;
\end{gathered}
$$

Выпишем формулы
$$
\begin{gathered}

\bar{M}_{1,2,3} = M_{4,5,6} =  B_1^3;\\
\bar{M}_{1,2,6} = M_{3,4,5} =  A_1 B_1^2;\\
\bar{M}_{1,3,5} = M_{2,4,6} = -A_1 B_1^2; \\
\bar{M}_{2,3,4} = M_{1,5,6} =  A_1 B_1^2;\\
\bar{M}_{1,5,6} = M_{2,3,4} =  A_1^2 B_1;\\
\bar{M}_{2,4,6} = M_{1,3,5} = -A_1^2 B_1;\\
\bar{M}_{3,4,5} = M_{1,2,6} =  A_1^2 B_1;\\
\bar{M}_{4,5,6} = M_{1,2,3} =  A_1 ^3;\\

\bar{M}_{1,3,6} = M_{2,4,5} = -B_1(A_1 B_2 - A_2 B_1);\\
\bar{M}_{2,3,5} = M_{1,4,6} =  B_1(A_1 B_2 - A_2 B_1);\\
\bar{M}_{2,5,6} = M_{1,3,4} = -A_1(A_1 B_2 - A_2 B_1);\\
\bar{M}_{3,4,6} = M_{1,2,5} =  A_1(A_1 B_2 - A_2 B_1);\\
\bar{M}_{2,3,6} = M_{1,4,5} =  A_1(B_2^2 - B_1 B_3) - B_1(A_2 B_2 - A_3 B_1);\\
\bar{M}_{3,5,6} = M_{1,2,4} =  A_1(A_1 B_3 - A_2 B_2) + B_1(A_2^2 - A_1 A_3);\\
\end{gathered}
$$

Найдены закономерности
$$
\begin{gathered}

\bar{M}_{1,2,3} = M_{4,5,6} =  B_1^3;\\
\bar{M}_{1,2,6} = M_{3,4,5} =  A_1 B_1^2;\\
\bar{M}_{1,5,6} = M_{2,3,4} =  A_1^2 B_1;\\
\bar{M}_{4,5,6} = M_{1,2,3} =  A_1^3;\\
\bar{M}_{1,3,5} = M_{2,4,6} = -M_{3,4,5}; \\
\bar{M}_{2,3,4} = M_{1,5,6} =  M_{3,4,5};\\
\bar{M}_{2,4,6} = M_{1,3,5} = -M_{2,3,4};\\
\bar{M}_{3,4,5} = M_{1,2,6} =  M_{2,3,4};\\

\bar{M}_{2,3,5} = M_{1,4,6} =  B_1(A_1 B_2 - A_2 B_1);\\
\bar{M}_{3,4,6} = M_{1,2,5} =  A_1(A_1 B_2 - A_2 B_1);\\
\bar{M}_{1,3,6} = M_{2,4,5} = -M_{1,4,6};\\
\bar{M}_{2,5,6} = M_{1,3,4} = -M_{1,2,5};\\

\bar{M}_{2,3,6} = M_{1,4,5} =  A_1(B_2^2 - B_1 B_3) - B_1(A_2 B_2 - A_3 B_1);\\
\bar{M}_{3,5,6} = M_{1,2,4} =  A_1(A_1 B_3 - A_2 B_2) + B_1(A_2^2 - A_1 A_3);\\
\end{gathered}
$$
