# Quadrat

Представление квадратичной кривой через кубическую

$$P_{2,Q} = P_{3,C}$$

$$\left\{
\begin{gathered}
	C_0 = Q_0,\\
	C_1 = Q_0+\frac{2 (Q_1 - Q_0)}{3},\\
	C_2 = Q_1+\frac{(Q_2 - Q_1)}{3},\\
	C_3 = Q_2;
\end{gathered}
\right.
$$

Это можно представить как:

$$\left\{
\begin{gathered}
	C_0 = Q_0,\\
	C_1 = Q_0+\frac{2 (Q_1 - Q_0)}{3},\\
	C_2 = Q_2+\frac{2 (Q_1 - Q_2)}{3},\\
	C_3 = Q_2;
\end{gathered}
\right.
$$

$$\left\{
\begin{gathered}
	C_0 = Q_0,\\
	C_1 = \frac{Q_0 + 2Q_1}{3},\\
	C_2 = \frac{Q_2 + 2Q_1}{3},\\
	C_3 = Q_2;
\end{gathered}
\right.
$$
