## Закономерности алгебраических сумм

Сдвиг пределов
$$\sum_{n=s}^{t} f(n) = \sum_{n=s+p}^{t+p} f(n-p).$$

Вынос члена
$$\sum_{n=s}^{t} f(n) = f(s) + \sum_{n=s+1}^{t} f(n).$$

Разложение чётных и нечётных пределов
$$\sum_{2s}^{2t+1} f(n) = \sum_{n=s}^t f(2n) + \sum_{n=s}^t f(2n+1);$$
$$\sum_{n=2s+1}^{2t} f(n) = \sum_{n=s+1}^t f(2n) + \sum_{n=s+1}^t f(2n-1).$$

Для $s=0$:
$$\sum_{k=0}^{2t+1} f(k) = \sum_{k=0}^t f(2k) + \sum_{k=0}^t f(2k+1);$$
$$\sum_{k=1}^{2t}   f(k) = \sum_{k=1}^t f(2k) + \sum_{k=1}^t f(2k-1).$$


$$\sum_{j=0}^{3} f(j) = \sum_{j_0=0}^1 \sum_{j_1=0}^1 f(2j_1+j_0).$$

$$\sum_{i=a}^{b+c} f(i) = \sum_{i=a}^{b-1} f(i} + \sum_{i=b}^{c} f(i).$$

$$\sum_{i=0}^{mn-1} f(i) = \sum_{j=0}^{m} \sum_{k=0}^{n-1} f(nj+k).$$


### По основанию 4

$$4n = 2(2n);\; 4n+1 = 2(2n) + 1;\; 4n+2 = 2(2n+1);\; 4n+3 = 2(2n+1) + 1.$$
$$4n = 2(2n);\; 4n-1 = 2(2n) - 1;\; 4n-2 = 2(2n-1);\; 4n-3 = 2(2n-1) - 1.$$

#### $4n$

$$\sum_{k=0}^{4n} f(k) 
= f(0) + \sum_{k=1}^{2(2n)} f(k)
= f(0) + \sum_{k=1}^{2n} f(2k) + \sum_{k=1}^{2n} f(2k-1);
$$

Обозначим
$$f(2k) = g_0(k);\ f(2k-1) = g_-(k);$$

$$\sum_{k=0}^{4n} f(k) 
= f(0) + \sum_{k=1}^{2n} g_0(k) + \sum_{k=1}^{2n} g_-(k)
= f(0) 
+\sum_{k=1}^n g_0(2k) + \sum_{k=1}^n g_0(2k-1) 
+\sum_{k=1}^n g_-(2k) + \sum_{k=1}^n g_-(2k-1)
;
$$


$$\sum_{k=0}^{4n} f(k) 
= f(0) 
+\sum_{k=1}^n f(2(2k)) 
+\sum_{k=1}^n f(2(2k-1)) 
+\sum_{k=1}^n f(2(2k)-1) 
+\sum_{k=1}^n f(2(2k-1)-1)
;$$

$$\sum_{k=0}^{4n} f(k) 
= f(0) 
+\sum_{k=1}^n 
\left(
 f(4k-3)
+f(4k-2) 
+f(4k-1) 
+f(4k)
\right)
.$$

$$\sum_{k=0}^{4n} f(k) 
= f(0) +
\sum_{k=1}^n 
\sum_{j=-3}^{0}
f(4k+j)
.$$

$$\sum_{k=0}^{4n} f(k) 
= f(0) +
\sum_{j=0}^{3}
\sum_{k=1}^n 
f(4k+j-3)
.$$


#### $4n+1$
$$\sum_{k=0}^{4n+1} f(k) = \sum_{k=0}^{2(2n)+1} f(k)
= \sum_{k=0}^{2n} f(2k) + \sum_{k=0}^{2n} f(2k+1)
;$$

Обозначим
$$f(2k) = g_0(k);\ f(2k+1) = g_+(k);$$

$$\sum_{k=0}^{4n+1} f(k) 
= \sum_{k=0}^{2n} g_0(k) + \sum_{k=0}^{2n} g_+(k)
= g_0(0) + \sum_{k=1}^{2n} g_0(k) 
+g_+(0) + \sum_{k=1}^{2n} g_+(k)
;$$

$$\sum_{k=0}^{4n+1} f(k) 
= g_0(0) + g_+(0) 
+\sum_{k=1}^n g_0(2k) 
+\sum_{k=1}^n g_0(2k-1)
+\sum_{k=1}^n g_+(2k) 
+\sum_{k=1}^n g_+(2k-1)
;$$

$$\sum_{k=0}^{4n+1} f(k) 
= f(0) + f(1) 
+\sum_{k=1}^n f(2(2k)) 
+\sum_{k=1}^n f(2(2k-1))
+\sum_{k=1}^n f(2(2k)+1) 
+\sum_{k=1}^n f(2(2k-1)+1)
;$$

$$\sum_{k=0}^{4n+1} f(k) 
= f(0) + f(1) 
+\sum_{k=1}^n 
\left(
 f(4k-2)
+f(4k-1)
+f(4k) 
+f(4k+1) 
\right)
.$$

$$\sum_{k=0}^{4n+1} f(k) 
= f(0) + f(1) +
\sum_{k=1}^n 
\sum_{j=-2}^{1} 
f(4k+j)
.$$

$$\sum_{k=0}^{4n+1} f(k) 
= f(0) + f(1) +
\sum_{j=0}^{3} 
\sum_{k=1}^n 
f(4k+j-2)
.$$

#### $4n+2$
$$\sum_{k=0}^{4n+2} f(k) = \sum_{k=0}^{2(2n+1)} f(k)
= f(0) + \sum_{k=1}^{2(2n+1)} f(k)
= f(0) + \sum_{k=1}^{2n+1} f(2k) + \sum_{k=1}^{2n+1} f(2k-1);
$$
Применим замены
$$\sum_{k=0}^{4n+2} f(k)
= f(0) + \sum_{k=1}^{2n+1} g_0(k) + \sum_{k=1}^{2n+1} g_-(k);
$$
Сдвинем пределы на -1:
$$\sum_{k=0}^{4n+2} f(k) 
= f(0) + \sum_{k=0}^{2n} g_0(k+1) + \sum_{k=0}^{2n} g_-(k+1)
= f(0) + g_0(1) + \sum_{k=1}^{2n} g_0(k+1) + g_-(1) + \sum_{k=1}^{2n} g_-(k+1);$$

$$\sum_{k=0}^{4n+2} f(k) 
= f(0) + f(1) + f(2) 
+\sum_{k=1}^{2n} g_0(k+1) 
+\sum_{k=1}^{2n} g_-(k+1)
;
$$

Введём новые замены
$$h_0(k) = g_0(k+1);\; h_-(k) = g_-(k+1);$$

$$\sum_{k=0}^{4n+2} f(k) 
= f(0) + f(1) + f(2) 
+\sum_{k=1}^{2n} h_0(k) 
+\sum_{k=1}^{2n} h_-(k)
= f(0) + f(1) + f(2) 
+\sum_{k=1}^n h_0(2k) 
+\sum_{k=1}^n h_0(2k-1)
+\sum_{k=1}^n h_-(2k) 
+\sum_{k=1}^n h_-(2k-1)
;
$$

$$\sum_{k=0}^{4n+2} f(k) 
= f(0) + f(1) + f(2) 
+\sum_{k=1}^n 
\left(
 g_0((2k)+1) 
+g_0((2k-1)+1)
+g_-((2k)+1) 
+g_-((2k-1)+1)
\right)
;
$$

$$\sum_{k=0}^{4n+2} f(k) 
= f(0) + f(1) + f(2) 
+\sum_{k=1}^n 
\left(
 f(2((2k)+1)) 
+f(2((2k-1)+1))
+f(2((2k)+1)-1) 
+f(2((2k-1)+1)-1)
\right)
;
$$

$$\sum_{k=0}^{4n+2} f(k) 
= f(0) + f(1) + f(2) 
+\sum_{k=1}^n 
\left(
 f(4k-1)
+f(4k)
+f(4k+1) 
+f(4k+2) 
\right)
.
$$

$$\sum_{k=0}^{4n+2} f(k) 
= f(0) + f(1) + f(2) +
\sum_{k=1}^n 
\sum_{j=-1}^{2} 
f(4k+j)
.$$

$$\sum_{k=0}^{4n+2} f(k) 
= f(0) + f(1) + f(2) +
\sum_{j=0}^{3} 
\sum_{k=1}^n 
f(4k+j-1)
.$$

#### $4n+3$
$$\sum_{k=0}^{4n+3} f(k)
= \sum_{k=0}^{2(2n+1)+1} f(k)
= \sum_{k=0}^{2n+1} f(2k) + \sum_{k=0}^{2n+1} f(2k+1)
= \sum_{k=0}^{2n+1} g_0(k) + \sum_{k=0}^{2n+1} g_+(k);
$$

$$\sum_{k=0}^{4n+3} f(k)
=
 \sum_{k=0}^n g_0(2k) 
+\sum_{k=0}^n g_0(2k+1)
+\sum_{k=0}^n g_+(2k) 
+\sum_{k=0}^n g_+(2k+1);
$$

$$\sum_{k=0}^{4n+3} f(k)
=
\sum_{k=0}^n 
\left(
 g_0(2k) 
+g_0(2k+1)
+g_+(2k) 
+g_+(2k+1)
\right);
$$

$$\sum_{k=0}^{4n+3} f(k)
=
\sum_{k=0}^n 
\left(
 f(2(2k)) 
+f(2(2k+1))
+f(2(2k)+1) 
+f(2(2k+1)+1)
\right);
$$

$$\sum_{k=0}^{4n+3} f(k)
=
\sum_{k=0}^n 
\left(
 f(4k) 
+f(4k+1) 
+f(4k+2)
+f(4k+3)
\right).
$$

$$\sum_{k=0}^{4n+3} f(k) = 
\sum_{k=0}^n 
\sum_{j=0}^{3} 
f(4k+j)
.$$

$$\sum_{k=0}^{4n+3} f(k) = 
\sum_{j=0}^{3} 
\sum_{k=0}^n 
f(4k+j)
.$$

### Результат


$$\sum_{k=0}^{4n+3} f(k) = 
\sum_{j=0}^{3} 
\sum_{k=0}^n 
f(4k+j)
.$$

$$\sum_{k=0}^{4n} f(k) 
= f(0) +
\sum_{j=0}^{3}
\sum_{k=1}^n 
f(4k+j-3)
.$$

$$\sum_{k=0}^{4n+1} f(k) 
= f(0) + f(1) +
\sum_{j=0}^{3} 
\sum_{k=1}^n 
f(4k+j-2)
.$$

$$\sum_{k=0}^{4n+2} f(k) 
= f(0) + f(1) + f(2) +
\sum_{j=0}^{3} 
\sum_{k=1}^n 
f(4k+j-1)
.$$
